src/Framework/Simulation/RefinementLift.v
@@ -13,12 +13,12 @@ Section RefinementLift.
     exact (Bind (compile T p2) (fun x => compile T' (p x))).
   Defined.
 
-  Fixpoint oracle_refines_to T u (d1: state L_imp) (p: prog L_abs T) get_reboot_state_imp o1 o2 : Prop :=
+  Fixpoint oracle_refines T u (d1: state L_imp) (p: prog L_abs T) get_reboot_state_imp o1 o2 : Prop :=
     match p with    
     |Op _ op =>
      exists o2',
      o2 =  [OpToken C_abs o2'] /\
-       CoreRefinement.(token_refines_to) u d1 op get_reboot_state_imp o1 o2'
+       CoreRefinement.(token_refines) u d1 op get_reboot_state_imp o1 o2'
     | Ret v =>
       (exists d1',
          exec L_imp u o1 d1 (Ret v) (Crashed d1') /\
@@ -32,20 +32,20 @@ Section RefinementLift.
       o1 = o1'++o1'' /\
       o2 = o2' ++ o2'' /\
      ((exists d1', exec L_imp u o1' d1 (compile T1 p1) (Crashed d1') /\
-         oracle_refines_to T1 u d1 p1 get_reboot_state_imp o1' o2') \/
+         oracle_refines T1 u d1 p1 get_reboot_state_imp o1' o2') \/
       (exists d1' r ret,
          exec L_imp u o1' d1 (compile T1 p1) (Finished d1' r) /\
          exec L_imp u o1'' d1' (compile T2 (p2 r)) ret /\
-         oracle_refines_to T1 u d1 p1 (fun s => s) o1' o2' /\
-         oracle_refines_to T2 u d1' (p2 r) get_reboot_state_imp o1'' o2''
+         oracle_refines T1 u d1 p1 (fun s => s) o1' o2' /\
+         oracle_refines T2 u d1' (p2 r) get_reboot_state_imp o1'' o2''
          ))
     end.
 
   Theorem exec_compiled_preserves_refinement_finished:
     forall T (p: L_abs.(prog) T) o s_imp s_imp' r u,
-      (exists s_abs, CoreRefinement.(refines_to_core) s_imp s_abs) ->
+      (exists s_abs, CoreRefinement.(refines_core) s_imp s_abs) ->
       L_imp.(exec) u o s_imp (compile T p) (Finished s_imp' r) ->
-      (exists s_abs', CoreRefinement.(refines_to_core) s_imp' s_abs').
+      (exists s_abs', CoreRefinement.(refines_core) s_imp' s_abs').
   Proof.
     induction p; simpl; intros;
     try invert_exec; eauto;
@@ -55,14 +55,14 @@ Section RefinementLift.
   (*
   Theorem exec_compiled_preserves_refinement_crashed:
     forall T (p: L_abs.(prog) T) o s_imp s_imp',
-      (exists s_abs, CoreRefinement.(refines_to_core) s_imp s_abs) ->
+      (exists s_abs, CoreRefinement.(refines_core) s_imp s_abs) ->
       L_imp.(exec) o s_imp (compile T p) (Crashed s_imp') ->
-      (exists s_abs', CoreRefinement.(refines_to_crash_core) s_imp' s_abs').
+      (exists s_abs', CoreRefinement.(refines_crash_core) s_imp' s_abs').
   Proof.
     induction p; simpl; intros;
     try invert_exec; eauto;
     try solve [eapply CoreRefinement.(exec_compiled_preserves_refinement_crashed_core); eauto].
-    apply refines_to_then_refines_to_crash_core; eauto.
+    apply refines_then_refines_crash_core; eauto.
     split_ors; cleanup; eauto.
     eapply exec_compiled_preserves_refinement_finished in H1; eauto.
   Qed.
@@ -70,8 +70,8 @@ Section RefinementLift.
   Definition LiftRefinement : Refinement L_imp L_abs :=
     Build_Refinement
       compile
-      CoreRefinement.(refines_to_core)
-      oracle_refines_to
+      CoreRefinement.(refines_core)
+      oracle_refines
       exec_compiled_preserves_refinement_finished.
 
 End RefinementLift.
